changing to new word representation

machine.v
@@ -1,57 +1,116 @@
 Require Import Omega.
-(* Our formalization uses bits to reflect actual computing hardware,
-but one could define a digits type in lieu of bits and redefine the
-below bytes data-type to use that digits type and the rest of the
-formalization (and critically all well-written MIX programs!) should
-be fine. *)
-Inductive bit : Type :=
-| zero : bit
-| one : bit.
+Require Import Finite.
+From RecordUpdate Require Import RecordSet.
+Require Import Types.
+Import MixWord.
 
-(* Bytes are comprised of 6 bits. They can therefore hold values from
-0 to 99, but we assume that bytes only hold 64 distinct values from
-(i.e. values from 0 to 63) *)
-Definition byte : Type := bit * bit * bit * bit * bit * bit.
+Inductive reg : Type :=
+    (* general purpose *)
+    rA | rX
+    (* index registers *)
+    | rI1 | rI2 | rI3 | rI4 | rI5 | rI6
+    (* jump register *)
+    | rJ.
 
-Inductive sign : Type :=
-| plus : sign
-| minus : sign.
+Module Type Registers.
+  Context (registers : Type).
+  Context (zeroRegisters : registers).
+  Context (getReg : registers -> reg -> word).
+  Context (setReg : registers -> reg -> word -> registers).
+End Registers.
 
-(* MIX words are comprised of a sign bit and 5 bytes *)
-Definition word : Type := sign * byte * byte * byte * byte * byte.
+Module MixRegisters : Registers.
+  (* Dumb coq bug: the kernel won't let you instantiate a parameter
+     with an record type (nor with an inductive definition)
+     directly. *)
+  Record registers' : Type := mkRegisters 
+                               {
+                                 (* Accumulator: "...has many uses,
+                                    especially for arithmetic and operating
+                                    on data." *)
+                                 A : word
+                                 (* Extension register: "...an extension
+                                    on the 'right-hand side' of rA, and it
+                                    is is used in conjuction with rA to hold
+                                    ten bytes of a product or dividend, or
+                                    it can be used to hold information
+                                    shifted to the right out of A." *)
+                                 ; X : word
+                                 (* Index registers comprised of a sign
+                                    and two bytes: "...used primarily for
+                                    for counting and for referencing
+                                    variable memory addresses." *)
+                                 ; I1 : sign * byte * byte
+                                 ; I2 : sign * byte * byte
+                                 ; I3 : sign * byte * byte
+                                 ; I4 : sign * byte * byte
+                                 ; I5 : sign * byte * byte
+                                 ; I6 : sign * byte * byte
+                                 (* Jump register comprised of two bytes
+                                    and (TODO?) a sign, where the sign is
+                                    always considered positive: "...always
+                                    holds the address of the instruction
+                                    following the most recent 'jump'
+                                    operation, and it is primarily used in
+                                    connection with subroutines." *)
+                                 ; J : byte * byte
+                               }.
+  Definition registers : Type := registers'.
 
-Record registers : Type := mkRegisters 
-                            {
-                              (* Accumulator: "...has many uses,
-                               especially for arithmetic and operating
-                               on data." *)
-                              A : word
-                              (* Extension register: "...an extension
-                              on the 'right-hand side' of rA, and it
-                              is is used in conjuction with rA to hold
-                              ten bytes of a product or dividend, or
-                              it can be used to hold information
-                              shifted to the right out of A." *)
-                              ; X : word
-                              (* Index registers comprised of a sign
-                                 and two bytes: "...used primarily for
-                                 for counting and for referencing
-                                 variable memory addresses." *)
-                              ; I1 : sign * byte * byte
-                              ; I2 : sign * byte * byte
-                              ; I3 : sign * byte * byte
-                              ; I4 : sign * byte * byte
-                              ; I5 : sign * byte * byte
-                              ; I6 : sign * byte * byte
-                              (* Jump register comprised of two bytes
-                              and (TODO?) a sign, where the sign is
-                              always considered positive: "...always
-                              holds the address of the instruction
-                              following the most recent 'jump'
-                              operation, and it is primarily used in
-                              connection with subroutines." *)
-                              ; J : byte * byte
-                            }.
+  (* For record updates *)
+  Instance etaRegisters : Settable _ := settable! mkRegisters <A; X; I1; I2; I3; I4; I5; I6; J>.
+
+  Definition zeroRegisters : registers := {| A := zero_word;
+                                             X := zero_word;
+                                             I1 := (plus , zero_byte , zero_byte);
+                                             I2 := (plus , zero_byte , zero_byte);
+                                             I3 := (plus , zero_byte , zero_byte);
+                                             I4 := (plus , zero_byte , zero_byte);
+                                             I5 := (plus , zero_byte , zero_byte);
+                                             I6 := (plus , zero_byte , zero_byte);
+                                             J := (zero_byte , zero_byte); |}.
+  
+
+  
+  Definition getReg (R : registers) (r : reg) : word + (sign * byte * byte) + (byte * byte) :=
+    match r with
+    | rA => inl (inl (A R))
+    | rX => inl (inl (X R))
+    | rI1 => inl (inr (I1 R))
+    | rI2 => inl (inr (I2 R))
+    | rI3 => inl (inr (I3 R))
+    | rI4 => inl (inr (I4 R))
+    | rI5 => inl (inr (I5 R))
+    | rI6 => inl (inr (I6 R))
+    | rJ => inr (J R)
+    end.
+  
+  Import RecordSetNotations.
+  Definition setReg (R : registers) (r : reg) (w : word + (sign * byte * byte) + (byte * byte) ) : registers :=
+    match w with
+    | inl (inl w) =>
+      match r with
+      | rA => R <|A := w|>
+      | rX => R <|X := w|>
+      | otherwise => R
+      end
+    | inl (inr s) =>
+      match r with
+        | rI1 => R <|I1 := s|>
+        | rI2 => R <|I2 := s|>
+        | rI3 => R <|I3 := s|>
+        | rI4 => R <|I4 := s|>
+        | rI5 => R <|I5 := s|>
+        | rI6 => R <|I6 := s|>
+        | _ => R
+      end
+    | inr s =>
+      match r with
+      | rJ => R <|J := s|>
+      | _ => R
+      end
+    end.
+End MixRegisters.
 
 Record flags : Type := mkFlags 
                          {
@@ -61,36 +120,215 @@ Record flags : Type := mkFlags
                               some lemmas maybe. *)
                            comparison : comparison
                            (* overflow bit that is set on or off
-                           depending on the outcome of an arithmetic
-                           instruction *)
+                              depending on the outcome of an
+                              arithmetic instruction *)
                            ; overflow : bit
                          }.
 
-(* finite types from autosubst2, used in defining memory as a finite map *)
-Fixpoint fin (n : nat) : Type :=
-  match n with
-  | 0 => False
-  | S m => option (fin m)
-  end.
+Definition zeroFlags : flags := {| comparison := Eq;
+                                   overflow := zero; |}.
 
-(* This is hard to define, let's just assume we can use it for now.
-   With a proof that n > 0, m < n, we get back the mth inhabitant of
-   the nth fintype. *)
-Hint Resolve Some.
-Hint Resolve None.
-Fixpoint fin_m_n {n : nat} (m : nat) (H: n > 0) (H': m < n) : fin n.
-Admitted.
+Context (size : nat).
+Context (Hsizenontrivial : size > 0).
 
-(* Each MIX machine has a 4000-word of memory. We represent this in
-Coq as a finite map from a type with 4000 inhabitants to words. *)
-Definition memory : Type := fin 4000 -> word.
+Definition address : Type := fin size.
 
-Lemma memgtz : 4000 > 0.
+Module Type Memory.
+  Context {size : nat}.
+  Context (memory : Type).
+  Context (zeroMemory : memory).
+  Context (HMemNontrivial : size > 0).
+  Context (get_nth_cell : memory -> {n : nat | n < size} -> word).
+  Context (set_nth_cell : memory -> {n : nat | n < size} -> word -> memory).
+  Notation " M [ n ] " := (get_nth_cell M n) (at level 50).
+End Memory.
+
+Module MixMemory : Memory.
+  (* Each MIX machine has a 4000-word memory. We represent this in
+     Coq as a finite map from a type with 4000 inhabitants to words. *)
+  Definition size := size.
+  Definition memory := fin size -> word.
+  Definition zeroMemory : memory := fun n => zero_word.
+  Definition HMemNontrivial : size > 0.
+    exact Hsizenontrivial.
+  Defined.
+  Definition mem_index (n : {n : nat | n < size}) : fin size := fin_n_m size n.
+  Definition get_nth_cell M (n : {n : nat | n < size}) : word :=
+    M (mem_index n).
+  Definition set_nth_cell M (n : {n : nat | n < size}) (w : word) : memory :=
+    (fun m : fin size => if fin_dec m (mem_index n) then w else M m).
+End MixMemory.
+
+(* Knuth uses ':' but we depart from this and get similar aesthetics
+   by squinting at Coq's pair syntax *)
+Definition fieldspec : Type := {L : nat | L < 6} * {R : nat | R < 6}.
+Definition fieldspecToNat (F : fieldspec) : {n : nat | n < 64}.
+  refine (exist _ (let (L', R') := F
+                   in match L' with 
+                      | exist _ L _ =>
+                                    match R' with 
+                                    | exist _ R _ => 8 * L + R
+                                    end
+                      end) _).
+  unfold fieldspec in F.
+  destruct F.
+  destruct s, s0.
   omega.
-Qed.
+Defined.
 
+Open Scope list_scope.
 
-Definition get_nth_cell (M : memory) (n : nat) {H : n < 4000} : word :=
-  M (fin_m_n n memgtz H).
+Definition fieldspecToByte F := natToByte (fieldspecToNat F).
 
-Notation " M [ n ] pf " := (get_nth_cell M n) (at level 50).
+Import MixRegisters.
+
+Inductive instruction : Type :=
+(** * Loads and stores *)
+(* Load a word (or part of it depending on the fieldspec), optionally
+negating it using a negative sign, into a given register from a given
+memory address possibly augmented by the value in a given index
+register. *)
+| Load : sign -> reg -> address -> option reg -> option fieldspec -> instruction
+| Store : reg -> address -> option fieldspec -> instruction
+| StoreZero : address -> option fieldspec -> instruction
+                                             
+(** * Arithmetic *)                                            
+| Add : address -> option fieldspec -> instruction
+| Sub : address -> option fieldspec -> instruction
+| Mul : address -> option fieldspec -> instruction
+| Div : address -> option fieldspec -> instruction
+                                       
+(** * Address transfer operations *)
+(* Enter a word, optionally negating it and optionally adjusted by the value in a given index register, into a register *)
+| Ent : sign -> reg -> word -> option reg -> instruction
+(* increase the value contained in a given register by a given word *)
+| Inc : reg -> word -> instruction
+(* decrease the value contained in a given register by a given word *)
+| Dec : reg -> word -> instruction
+
+(** * Comparison operators *)
+| Cmp : reg -> address -> fieldspec -> instruction
+
+(** * Jump operators *)
+(* unconditional jump *)
+| Jmp : address -> instruction
+(* unconditional jump that doesn't update the jump register *)
+| Jsj : address -> instruction
+(* conditionally jump if there has been an overflow *)
+| Jov : address -> instruction
+(* conditionally jump if there hasn't been an overflow *)
+| Jnov : address -> instruction
+(* jump on less, equal, greater, greater-or-equal, unequal,
+   less-or-equal comparison flags respectively *)
+| Jl : address -> instruction
+| Je : address -> instruction
+| Jg : address -> instruction
+| Jge : address -> instruction
+| Jne : address -> instruction
+| Jle : address -> instruction
+(* jump on register negative, zero, positive, nonnegative, nonzero,
+   nonpositive respectively *)
+| Jrn : reg -> address -> instruction
+| Jrz : reg -> address -> instruction
+| Jrp : reg -> address -> instruction
+| Jrnn : reg -> address -> instruction
+| Jrnz : reg -> address -> instruction
+| Jrnp : reg -> address -> instruction
+
+(** * Miscellaneous operators *)
+(** shifts *)
+(* Shift a given register left or right by a given number of bytes *)
+| Sl : reg -> word -> instruction
+| Sr : reg -> word -> instruction
+(* special AX-shifts *)
+| Slax : word -> instruction
+| Srax : word -> instruction
+(* circular AX-shifts *)
+| Slc : word -> instruction
+| Src : word -> instruction
+
+(* Move the number of words specified by the fieldspec from location M
+   to the location specified by the contents of I1 *)
+| Move : address -> fieldspec -> instruction
+
+(* no-op *)
+| Nop : instruction
+(* halt the machine *)
+| Hlt : instruction
+          
+(** * TODO: IO operators *)
+(* Need to decide on how much I want to model this and how to do so *)
+          
+(** * TODO: Conversion operators *)
+(* Left for later due to laziness *).
+
+Import MixMemory.
+
+Record machine : Type := mkMachine {
+                             r : registers;
+                             f : flags;
+                             m : memory
+                           }.
+
+Definition zeroMachine : machine := {| r := zeroRegisters;
+                                       f := zeroFlags;
+                                       m := zeroMemory |}.
+
+Inductive indexRegister : reg -> Prop :=
+  | indexI1 : indexRegister rI1
+  | indexI2 : indexRegister rI2
+  | indexI3 : indexRegister rI3
+  | indexI4 : indexRegister rI4
+  | indexI5 : indexRegister rI5
+  | indexI6 : indexRegister rI6.
+
+Inductive instWf : instruction -> Prop :=
+| LoadWf : forall sign rDest from maybeIndex I maybeFieldspec,
+    (maybeIndex = Some(I) -> indexRegister I) ->
+    instWf (Load sign rDest from maybeIndex maybeFieldspec)
+| HaltWf : instWf Hlt.
+
+Definition instDenote (M : machine) (I : {I : instruction | instWf I}) : machine :=
+  let (I, _) := I in 
+    in match I with
+       | (Load sign rDest from maybeIndex maybeFieldspec, _) =>
+         match (maybeIndex, maybeFieldspec) with
+         | (Some(I), Some(F)) =>
+           (* offset from by the value contained in I *)
+           let offset := indexToNat (getReg I) in
+         | (Some(I), None) => 
+         | (None, Some(F)) =>
+         | (None, None) => 
+           let 
+             {| r := 
+                  f := M.f;
+                m := M.m;
+             |}
+           | otherwise => M
+             end.
+
+Definition Halto : {I : instruction | instWf I}.
+  econstructor.
+  instantiate (1 := Hlt).
+  auto.
+  constructor.
+  Defined.
+
+Compute instDenote zeroMachine Halto.
+
+  in match I with
+     | (Load sign rDest from maybeIndex maybeFieldspec, _) =>
+       match (maybeIndex, maybeFieldspec) with
+       | (Some(I), Some(F)) =>
+         (* offset from by the value contained in I *)
+         let offset := indexToNat (getReg I) in
+       | (Some(I), None) => 
+       | (None, Some(F)) =>
+       | (None, None) => 
+         let 
+           {| r := 
+                f := M.f;
+              m := M.m;
+           |}
+         | otherwise => M
+           end.
