Finite.v
@@ -1,0 +1,33 @@
+Require Import Omega.
+
+(* finite types used in defining memory as a finite map *)
+Fixpoint fin (n : nat) : Type :=
+  match n with
+  | 0 => False
+  | S m => option (fin m)
+  end.
+
+(* Decidable equality for finite types *)
+Definition fin_dec : forall {n} (f f' : fin n), ({f = f'} + {f <> f'}).
+  intros n f f'.
+  destruct n.
+  - inversion f.
+  -
+    destruct f.
+    destruct f'.
+Admitted.
+
+(* Get the mth element of the n-ary finite type *)
+Fixpoint fin_n_m (n : nat) (m : {m : nat | m < n}) : fin n.
+  destruct m.
+  destruct n.
+  - exfalso.
+    inversion l.
+  - destruct x.
+    + exact None.
+    +
+      apply Some.
+      apply fin_n_m.
+      assert (x < n) by omega.
+      exact (exist (fun m => m < n) x H).
+Defined.
