Registers.v
@@ -1,0 +1,101 @@
+From RecordUpdate Require Import RecordSet.
+
+Module Type Registers.
+  Context (registers : Type).
+  Context (zeroRegisters : registers).
+  Context (getReg : registers -> reg -> word + sign * byte * byte + byte * byte).
+  Context (setReg : registers -> reg -> word + sign * byte * byte + byte * byte -> registers).
+End Registers.
+
+Module MixRegisters : Registers.
+  (* Dumb coq bug: the kernel won't let you instantiate a parameter
+     with an record type (nor with an inductive definition)
+     directly. *)
+  Record registers' : Type := mkRegisters 
+                               {
+                                 (* Accumulator: "...has many uses,
+                                    especially for arithmetic and operating
+                                    on data." *)
+                                 A : word
+                                 (* Extension register: "...an extension
+                                    on the 'right-hand side' of rA, and it
+                                    is is used in conjuction with rA to hold
+                                    ten bytes of a product or dividend, or
+                                    it can be used to hold information
+                                    shifted to the right out of A." *)
+                                 ; X : word
+                                 (* Index registers comprised of a sign
+                                    and two bytes: "...used primarily for
+                                    for counting and for referencing
+                                    variable memory addresses." *)
+                                 ; I1 : sign * byte * byte
+                                 ; I2 : sign * byte * byte
+                                 ; I3 : sign * byte * byte
+                                 ; I4 : sign * byte * byte
+                                 ; I5 : sign * byte * byte
+                                 ; I6 : sign * byte * byte
+                                 (* Jump register comprised of two bytes
+                                    and (TODO?) a sign, where the sign is
+                                    always considered positive: "...always
+                                    holds the address of the instruction
+                                    following the most recent 'jump'
+                                    operation, and it is primarily used in
+                                    connection with subroutines." *)
+                                 ; J : byte * byte
+                               }.
+  Definition registers : Type := registers'.
+
+  (* For record updates *)
+  Instance etaRegisters : Settable _ := settable! mkRegisters <A; X; I1; I2; I3; I4; I5; I6; J>.
+
+  Definition zeroRegisters : registers := {| A := zero_word;
+                                             X := zero_word;
+                                             I1 := (plus , zero_byte , zero_byte);
+                                             I2 := (plus , zero_byte , zero_byte);
+                                             I3 := (plus , zero_byte , zero_byte);
+                                             I4 := (plus , zero_byte , zero_byte);
+                                             I5 := (plus , zero_byte , zero_byte);
+                                             I6 := (plus , zero_byte , zero_byte);
+                                             J := (zero_byte , zero_byte); |}.
+  
+
+  
+  Definition getReg (R : registers) (r : reg) : word + (sign * byte * byte) + (byte * byte) :=
+    match r with
+    | rA => inl (inl (A R))
+    | rX => inl (inl (X R))
+    | rI1 => inl (inr (I1 R))
+    | rI2 => inl (inr (I2 R))
+    | rI3 => inl (inr (I3 R))
+    | rI4 => inl (inr (I4 R))
+    | rI5 => inl (inr (I5 R))
+    | rI6 => inl (inr (I6 R))
+    | rJ => inr (J R)
+    end.
+  
+  Import RecordSetNotations.
+  Definition setReg (R : registers) (r : reg) (w : word + (sign * byte * byte) + (byte * byte) ) : registers :=
+    match w with
+    | inl (inl w) =>
+      match r with
+      | rA => R <|A := w|>
+      | rX => R <|X := w|>
+      | otherwise => R
+      end
+    | inl (inr s) =>
+      match r with
+        | rI1 => R <|I1 := s|>
+        | rI2 => R <|I2 := s|>
+        | rI3 => R <|I3 := s|>
+        | rI4 => R <|I4 := s|>
+        | rI5 => R <|I5 := s|>
+        | rI6 => R <|I6 := s|>
+        | _ => R
+      end
+    | inr s =>
+      match r with
+      | rJ => R <|J := s|>
+      | _ => R
+      end
+    end.
+End MixRegisters.
