Types.v
@@ -1,0 +1,95 @@
+Require Import Finite.
+Require Import Omega.
+
+Module Type Word.
+  Context (size : {n : nat | n > 0}).
+  Context (word : Type).
+  Context (signed : word -> Z).
+  Context (unsigned : word -> Z).
+  Context (fromZ : Z -> word).
+End Word.
+
+Module MixWord : Word.
+  Definition size : {n : nat | n > 0}. refine (exist _ 64 _); omega. Defined.
+  Definition word : Type := Z.
+  Open Scope Z_scope.
+  Let wrap := let (w, _) := size in Z.of_nat w.
+  (* Overflow doesn't change sign. Actually, Knuth is kind of vague
+  about the semantics of overflow in TAOCP, I suppose leaving it as
+  undefined behavior. *)
+  Definition signed (w : word) : Z :=
+    match w with
+    | Z0 => w
+    | Zpos x => w mod wrap
+    | Zneg x => - ((Zpos x) mod wrap)
+    end.
+
+  Definition unsigned (w : word) : Z :=
+    match w with
+    | Z0 => w
+    | Zpos x => w mod wrap
+    | Zneg x => (Zpos x) mod wrap
+    end.
+
+  Definition fromZ (z : Z) : word := id z.
+End MixWord.
+
+Definition zero_word := MixWord.fromZ 0.
+  
+(* (* Our formalization uses bits to reflect actual computing hardware, *)
+(*    but one could define a digits type in lieu of bits and redefine the *)
+(*    below bytes data-type to use that digits type and the rest of the *)
+(*    formalization (and critically all well-written MIX programs!) *)
+(*    should be fine. *) *)
+(*   Inductive bit : Type := *)
+(*   | one : bit *)
+(*   | zero : bit. *)
+
+(* (* Bytes are comprised of 6 bits. They can therefore hold values from *)
+(*    0 to 99, but we assume that bytes only hold 64 distinct values from *)
+(*    (i.e. values from 0 to 63) *) *)
+(*   Definition byte : Type := bit * bit * bit * bit * bit * bit. *)
+
+(*   Definition byteToNat (B : byte) : nat := *)
+(*     match B with *)
+(*     | (b5,b4,b3,b2,b1,b0) => *)
+(*       (if b5 then 2 ^ 5 else 0) + *)
+(*       (if b4 then 2 ^ 4 else 0) + *)
+(*       (if b3 then 2 ^ 3 else 0) + *)
+(*       (if b2 then 2 ^ 2 else 0) + *)
+(*       (if b1 then 2 ^ 1 else 0) + *)
+(*       (if b0 then 2 ^ 0 else 0) *)
+(*     end. *)
+
+(* Require Import Coq.Program.Wf. *)
+(* Program Fixpoint natToBits (n : nat) {wf lt n} : list bit := *)
+(*   match n with *)
+(*   | 0 => nil *)
+(*   | S n' => List.rev ((if (Nat.eq_dec (n mod 2) 0) then zero else one) :: natToBits (Nat.div2 n)) *)
+(*   end. *)
+(* Obligation 1. *)
+(* apply Nat.lt_div2. *)
+(* omega. *)
+(* Qed. *)
+
+(* Import List.ListNotations. *)
+(* Open Scope list_scope. *)
+(* Compute natToBits 11. *)
+
+(* Search "Z". *)
+
+(* (* MIX words are comprised of a sign bit and 5 bytes *) *)
+(* Definition word : Type := sign * byte * byte * byte * byte * byte. *)
+
+(* Definition nat_to_byte (n : {n : nat | n < 64}) : byte := fin_n_m 64 n. *)
+(* Definition byte_to_nat (b : byte) : {n : nat | n < 64} *)
+
+(* Definition zero_byte : byte. *)
+(*   apply n_byte. *)
+(*   econstructor. *)
+(*   instantiate (1 := 0). *)
+(*   abstract omega. *)
+(* Defined. *)
+       
+(* (* Definition zero_byte : byte := (zero , zero , zero , zero , zero , zero). *) *)
+(* Definition zero_word : word := (plus , zero_byte , zero_byte , zero_byte , zero_byte , zero_byte). *)
